Fix examples

pulse/examples/steel/arraystructs/ListNode.fst
@@ -5,45 +5,57 @@ module ListNode
 open FStar.FunctionalExtensionality
 module A = Steel.Effect.Atomic
 open Steel.Effect
-open FStar.PCM
 open Steel.C.Opt
 open Steel.C.PCM
 open Steel.C.Ref
 open Steel.C.Connection
 open Steel.C.Struct
 module U = FStar.Universe
+module P = FStar.PCM
 
 type node_field = | Value | Next
 
-let node_fields (node:Type u#1) k : Type u#1 = match k with
-  | Value -> option int'
+let node_fields (node:Type u#0) k : Type u#0 = match k with
+  | Value -> option int
   | Next -> option (option (ref' node node))
 
 #push-options "--__no_positivity"
-noeq type node: Type u#1 =
+noeq type node: Type u#0 =
 { un_node: restricted_t node_field (node_fields node) }
 #pop-options
 
-let node': Type u#1 = restricted_t node_field (node_fields node)
+let node': Type u#0 = restricted_t node_field (node_fields node)
 
 let node_fields_pcm k: pcm (node_fields node k) = match k with
-  | Value -> opt_pcm #int'
+  | Value -> opt_pcm #int
   | Next -> opt_pcm #(option (ref' node node))
 
 let node_pcm': pcm node' = prod_pcm node_fields_pcm
 
-let node_pcm: pcm node = {
-  FStar.PCM.p = {
-    composable = (fun x y -> composable node_pcm' x.un_node y.un_node);
-    op = (fun x y -> Mknode (op node_pcm' x.un_node y.un_node));
-    one = Mknode (one node_pcm');
+let node_composable
+  (x y: _)
+: Tot prop
+= composable node_pcm' x.un_node y.un_node
+
+let node_op
+  (x: _) (y: _ { node_composable x y })
+: Tot _
+= Mknode (op node_pcm' x.un_node y.un_node)
+
+let fstar_node_pcm: FStar.PCM.pcm node = {
+  P.p = {
+    P.composable = node_composable;
+    P.op = node_op;
+    P.one = Mknode (one node_pcm');
   };
-  comm = (fun x y -> node_pcm'.comm x.un_node y.un_node);
-  assoc = (fun x y z -> node_pcm'.assoc x.un_node y.un_node z.un_node);
-  assoc_r = (fun x y z -> node_pcm'.assoc_r x.un_node y.un_node z.un_node);
-  is_unit = (fun x -> node_pcm'.is_unit x.un_node);
-  refine = (fun x -> node_pcm'.refine x.un_node);
+  P.comm = (fun x y -> op_comm node_pcm' x.un_node y.un_node);
+  P.assoc = (fun x y z -> op_assoc_l node_pcm' x.un_node y.un_node z.un_node);
+  P.assoc_r = (fun x y z -> op_assoc_r node_pcm' x.un_node y.un_node z.un_node);
+  P.is_unit = (fun x -> is_unit node_pcm' x.un_node);
+  P.refine = (fun x -> p_refine node_pcm' x.un_node);
 }
+
+let node_pcm: pcm node = pcm_of_fstar_pcm fstar_node_pcm
 
 let roll: node_pcm' `morphism` node_pcm =
   mkmorphism
@@ -76,7 +88,7 @@ let roll_conn: node_pcm' `connection` node_pcm =
 let unroll_conn: node_pcm `connection` node_pcm' =
   connection_of_isomorphism node_iso
 
-let mk_node'_f (value: option int') (next: option (option (ref' node node)))
+let mk_node'_f (value: option int) (next: option (option (ref' node node)))
   (k: node_field)
 : node_fields node k
 = match k with
@@ -84,7 +96,7 @@ let mk_node'_f (value: option int') (next: option (option (ref' node node)))
   | Next -> next
   
 let mk_node'
-  (value: Ghost.erased (option int'))
+  (value: Ghost.erased (option int))
   (next: Ghost.erased (option (option (ref' node node))))
 : Ghost.erased node'
 = Ghost.hide (on_domain node_field (mk_node'_f (Ghost.reveal value) (Ghost.reveal next)))
@@ -92,15 +104,15 @@ let mk_node'
 let mk_node value next = Ghost.hide (Mknode (mk_node' (Ghost.reveal value) (Ghost.reveal next)))
 
 let _value
-: node_pcm `connection` opt_pcm #int'
+: node_pcm `connection` opt_pcm #int
 = unroll_conn `connection_compose` struct_field node_fields_pcm Value
 
 let _next
 : node_pcm `connection` opt_pcm #(option (ref' node node))
 = unroll_conn `connection_compose` struct_field node_fields_pcm Next
 
-let one_next : Ghost.erased (option int') =
-  Ghost.hide (one (opt_pcm #int'))
+let one_next : Ghost.erased (option int) =
+  Ghost.hide (one (opt_pcm #int))
 
 let node'_without_value value next
 : Lemma (struct_without_field node_fields_pcm Value (mk_node' value next) `feq`
@@ -133,17 +145,21 @@ let mk_node_mk_node' value next
 = ()
 
 let unroll_ref 
-  (#value:Ghost.erased (option int'))
+  (#value:Ghost.erased (option int))
   (#next:Ghost.erased (option (option (ref' node node))))
   (p: ref 'a node_pcm)
-: SteelT (p':ref 'a node_pcm'{p' == ref_focus p unroll_conn})
+: Steel (ref 'a node_pcm')
     (p `pts_to` mk_node value next)
     (fun p' -> p' `pts_to` mk_node' value next)
+    (requires (fun _ -> True))
+    (ensures (fun _ p' _ ->
+      p' == ref_focus p unroll_conn
+    ))
 = let p' = focus p unroll_conn (mk_node value next) (mk_node' value next) in
   A.return p'
 
 let roll_ref 
-  (#value:Ghost.erased (option int'))
+  (#value:Ghost.erased (option int))
   (#next:Ghost.erased (option (option (ref' node node))))
   (p: ref 'a node_pcm) (p': ref 'a node_pcm')
 : Steel unit
@@ -155,14 +171,18 @@ let roll_ref
   A.change_equal_slprop (p `pts_to` _) (p `pts_to` _)
 
 let addr_of_value
-  (#value:Ghost.erased (option int'))
+  (#value:Ghost.erased (option int))
   (#next:Ghost.erased (option (option (ref' node node))))
   (p: ref 'a node_pcm)
-: SteelT (q:ref 'a (opt_pcm #int'){q == ref_focus p _value})
+: Steel (q:ref 'a (opt_pcm #int))
     (p `pts_to` mk_node value next)
     (fun q ->
        (p `pts_to` mk_node none next) `star`
        (q `pts_to` value))
+    (requires (fun _ -> True))
+    (ensures (fun _ q _ ->
+      q == ref_focus p _value
+    ))
 = let p' = unroll_ref p in
   let q = addr_of_struct_field p' Value (mk_node' value next) in
   A.change_equal_slprop (p' `pts_to` _) (p' `pts_to` mk_node' none next);
@@ -171,13 +191,15 @@ let addr_of_value
   A.return q
 
 let unaddr_of_value
-  (#value:Ghost.erased (option int'))
+  (#value:Ghost.erased (option int))
   (#next:Ghost.erased (option (option (ref' node node))))
   (p: ref 'a node_pcm)
-  (q: ref 'a (opt_pcm #int'){q == ref_focus p _value})
-: SteelT unit
+  (q: ref 'a (opt_pcm #int))
+: Steel unit
     ((p `pts_to` mk_node none next) `star` (q `pts_to` value))
     (fun _ -> p `pts_to` mk_node value next)
+    (requires (fun _ -> q == ref_focus p _value))
+    (ensures (fun _ _ _ -> True))
 = let p' = unroll_ref p in
   let q = unaddr_of_struct_field Value q p' (mk_node' none next) value in
   A.change_equal_slprop (p' `pts_to` _) (p' `pts_to` mk_node' value next);
@@ -185,7 +207,7 @@ let unaddr_of_value
   A.return ()
 
 let addr_of_next
-  (#value:Ghost.erased (option int'))
+  (#value:Ghost.erased (option int))
   (#next:Ghost.erased (option (option (ref' node node))))
   (p: ref 'a node_pcm)
 : SteelT (q:ref 'a (opt_pcm #(option (ref' node node))){q == ref_focus p _next})
@@ -201,7 +223,7 @@ let addr_of_next
   A.return q
 
 let unaddr_of_next
-  (#value:Ghost.erased (option int'))
+  (#value:Ghost.erased (option int))
   (#next:Ghost.erased (option (option (ref' node node))))
   (p: ref 'a node_pcm)
   (q: ref 'a (opt_pcm #(option (ref' node node))){q == ref_focus p _next})
